chore: give up on fancy definitions, build raw circuits by hand
While I had a lot of nice theory, using it was too painful,
so I now opt to build the raw safety and related circuits "by hand",
and prove their correctness.

This is definitely much more low-level, but hopefully builds reusable,
black-box components which can be used further without the end-user
need to think or care about these definitions.

SSA/Experimental/Bits/Fast/FiniteStateMachine.lean
@@ -156,6 +156,10 @@ def eval' (x : arity → BitStream) : BitStream :=
 def changeInitCarry (p : FSM arity) (c : p.α → Bool) : FSM arity :=
   { p with initCarry := c }
 
+@[simp]
+theorem initCarry_changeInitCarry_eq (p : FSM arity) (c : p.α → Bool) :
+    (p.changeInitCarry c).initCarry = c := rfl
+
 theorem carry_changeInitCarry_succ
     (p : FSM arity) (c : p.α → Bool) (x : arity → BitStream) : ∀ n,
     (p.changeInitCarry c).carry x (n+1) =
@@ -179,26 +183,106 @@ theorem eval_eq_carry (x : arity → BitStream) (n : ℕ) :
     p.eval x n = (p.nextBit (p.carry x n) (fun i => x i n)).2 :=
   rfl
 
-/-- compute the next evaluation bit starting with 'initCarry'.
-TODO: write theorems for 'evalWith'.
--/
-def evalWith (p : FSM arity) (c : p.α → Bool) (x : arity → BitStream) : BitStream :=
-  (p.changeInitCarry c).eval x
-
 @[simp]
 theorem changeInitCarry_eq_self (p : FSM arity) :
     p.changeInitCarry p.initCarry = p := by
   simp [changeInitCarry]
 
+-- The actual API that theorems should be written is 'carryWith' and 'evalWith',
+-- since they describe the evolution of the FSM carry and output states.
+
+/-- compute the nth carry bits, starting with 'c', upto 'n' steps,
+for an input stream. -/
+def carryWith (p : FSM arity) (carryState : p.α → Bool) (x : arity → BitStream) (n : Nat) : p.α → Bool := fun a =>
+  (p.changeInitCarry carryState).carry x n a
+
+@[simp]
+theorem carryWith_zero_eq (carryState : p.α → Bool) (x : arity → BitStream) :
+    p.carryWith carryState x 0 =  carryState := by
+  ext s
+  simp [carryWith, changeInitCarry, carry]
+
+/-- One step transition of the FSM.-/
+def delta (p : FSM arity) (carryState : p.α → Bool) (x : arity → BitStream) : p.α → Bool :=
+  p.carryWith carryState x 1
+
+@[simp]
+theorem delta_eq_carryWith_one (carryState : p.α → Bool) (x : arity → BitStream) :
+    p.delta carryState x = p.carryWith carryState x 1 := rfl
+
+
+/--
+the 'carryWith' of the successor equals the 'carryWith' of the predecessor, with a different init state.
+-/
+@[simp]
+theorem carryWith_delta_eq_succ_carryWith (carryState : p.α → Bool) (x : arity → BitStream) :
+    p.carryWith (p.delta carryState x) (fun a i => x a (i + 1)) n =
+    p.carryWith carryState x (n + 1) := by
+  ext s
+  conv =>
+    rhs
+    rw [carryWith]
+  rw [carry_changeInitCarry_succ]
+  rw [← carryWith]
+  /- theorem to show is that 'carryWith of carryWith is compositional. -/
+  congr
+
+@[simp]
+theorem carryWith_carryWith_one_eq_succ_carryWith (carryState : p.α → Bool) (x : arity → BitStream) :
+    p.carryWith (p.carryWith carryState x 1) (fun a i => x a (i + 1)) n =
+    p.carryWith carryState x (n + 1) := by
+  ext s
+  conv =>
+    rhs
+    rw [carryWith]
+  rw [carry_changeInitCarry_succ]
+  rw [← carryWith]
+  congr
+
+
+theorem carryWith_carryWith_eq_carryWith (carryState : p.α → Bool) (x : arity → BitStream) :
+      p.carryWith (p.carryWith carryState x n) (fun a i => x a (n + i)) m =
+      p.carryWith carryState x (n + m) := by
+  induction n generalizing carryState x
+  case zero =>
+    simp
+  case succ n ih =>
+    sorry
+
+theorem carryWith_eq_carry_of_eq_initCarry (p : FSM arity) (carryState : p.α → Bool) (x : arity → BitStream) (n : Nat)
+    (hc : carryState = p.initCarry) :
+    p.carryWith carryState x n = p.carry x n := by
+  subst hc
+  ext s
+  simp [carryWith, changeInitCarry]
+
+@[simp]
+theorem carryWith_initCarry_eq_carry (p : FSM arity) (x : arity → BitStream) (n : Nat) :
+    p.carryWith p.initCarry x n = p.carry x n := by
+  ext s
+  simp [carryWith, changeInitCarry]
+
+
+/-- compute the next evaluation bit starting with 'initCarry'.
+TODO: write theorems for 'evalWith'.
+-/
+def evalWith (p : FSM arity) (carryState : p.α → Bool) (x : arity → BitStream) : BitStream :=
+  (p.changeInitCarry carryState).eval x
+
+/-- compute the output of the FSM, given the carry state and the environment of the immediate next bits. -/
+def outputWith (p : FSM arity) (carryState : p.α → Bool) (env : arity → Bool) : Bool :=
+  (p.nextBitCirc none).eval (Sum.elim carryState env)
+
 /-- evalWith agrees with eval when we set the carry to the init carry. -/
-theorem evalWith_eq_eval_of_eq_init (p : FSM arity) (c : p.α → Bool) (x : arity → BitStream)
-    (hc : c = p.initCarry) : p.evalWith c x = p.eval x := by
+theorem evalWith_eq_eval_of_eq_init (p : FSM arity) (carryState : p.α → Bool) (x : arity → BitStream)
+    (hc : carryState = p.initCarry) : p.evalWith carryState x = p.eval x := by
   simp [hc, evalWith]
 
 @[simp]
 theorem evalWith_initCarry_eq_init (p : FSM arity)
     : p.evalWith p.initCarry = p.eval := by
   ext x; simp [evalWith]
+
 
 /-- `p.changeVars f` changes the arity of an `FSM`.
 The function `f` determines how the new input bits map to the input expected by `p` -/
